update other blood and list class

verification/DisposedBlood.dfy
@@ -1,14 +1,15 @@
-class {:autocontracts} DisposedBlood {
+class DisposedBlood {
     var id: int;
 
-    predicate Valid()
+    /*predicate Valid()
     reads this
     {
         true
-    }
+    }*/
 
     constructor (bloodid: int)
     ensures id == bloodid
+    modifies this
     {
         id := bloodid;
     }
