verification/UntestedBlood.dfy
@@ -1,15 +1,16 @@
-class {:autocontracts} UntestedBlood {
+class UntestedBlood {
     var id: int;
     var retrieval:int;
 
-    predicate Valid()
+    /*predicate Valid()
     reads this
     {
         true
-    }
+    }*/
 
     constructor (bloodid: int, rdate: int)
     ensures id == bloodid && rdate == retrieval
+    modifies this
     {
         id := bloodid;
         retrieval := rdate;
