verification/TestingBlood.dfy
@@ -1,4 +1,4 @@
-class {:autocontracts} TestingBlood {
+class TestingBlood {
     var id: int;
     var retrieval: int;
     var startTest: int;
@@ -12,6 +12,8 @@ class {:autocontracts} TestingBlood {
     constructor (bloodid: int, rdate: int, sdate: int)
     requires sdate > rdate
     ensures id == bloodid && rdate == retrieval && sdate == startTest
+    modifies this
+    ensures Valid()
     {
         id := bloodid;
         retrieval := rdate;
